Main.lean
@@ -6,10 +6,10 @@ import IntroEffects
 open Input
 
 def printFullName := {{{
-  do _a ← print(str("What is your forename?"); fun y ↦ (return y)) in
-  do forename ← read((); fun y ↦ (return y)) in
-  do _b ← print(str("What is your surname?"); fun y ↦ (return y)) in
-  do surname ← read((); fun y ↦ (return y)) in
+  ← print⟨str "What is your forename?"⟩;
+  do forename ← read⟨()⟩ in
+  ← print⟨str "What is your surname?"⟩;
+  do surname ← read⟨()⟩ in
   do joined ← join(forename, surname) in
   return joined
 }}}
@@ -23,8 +23,71 @@ info: Bob Bob
 -/
 #guard_msgs in
 #evalLang {{{
-  do h ← ~alwaysRead str("Bob")  in
+  do h ← ~alwaysRead (str "Bob") in
   with h handle ~printFullName
+}}}
+
+def abc := {{{
+  ← print⟨str "A"⟩;
+  ← print⟨str "B"⟩;
+  print⟨str "C"⟩
+}}}
+
+def collect := {{{
+  handler {
+    return x ↦ return pair(x, str ""),
+    ops := [
+      "print"(s, k) ↦
+        do (x, acc) ← k () in
+        do joined ← join(s, acc) in
+        return pair(x, joined)
+    ]
+  }
+}}}
+
+/--
+info: ((), A B C )
+-/
+#guard_msgs in
+#evalLang {{{
+  with ~collect handle ~abc
+}}}
+
+def reverse := {{{
+  handler {
+    ops := ["print"(s,k) ↦ ← k (); print⟨s⟩]
+  }
+}}}
+
+/--
+info: ((), C B A )
+-/
+#guard_msgs in
+#evalLang {{{
+  with ~collect handle
+  with ~reverse handle ~abc
+}}}
+
+def collect' := {{{
+  handler {
+    return x ↦ return (fun acc ↦ (return pair(x, acc))),
+    ops := [
+      "print"(s, k) ↦
+        return (fun acc ↦
+          (do res ← k () in
+          do joined ← join(acc, s) in
+          res joined))
+    ]
+  }
+}}}
+
+/--
+info: ((),  A B C)
+-/
+#guard_msgs in
+#evalLang {{{
+  do f ← (with ~collect' handle ~abc) in
+  f (str "")
 }}}
 
 def main : IO Unit :=
